src/PredCalcEquivLemmas.v
@@ -110,146 +110,138 @@ Section props.
 
   (* A.22 *)
   Lemma f_imp_equiv_or A B :
-    <! A => B !> ≡ <! ¬ A ∨ B !>.
+    <! A ⇒ B !> ≡ <! ¬ A ∨ B !>.
   Proof. prove_equiv. Qed.
 
   (* A.23 *)
   Lemma f_implies_self A :
-    <! A => A !> ≡ <! true !>.
+    <! A ⇒ A !> ≡ <! true !>.
   Proof. prove_equiv. Qed.
 
   (* A.24 *)
   Lemma f_impl_as_not_and A B :
-    <! A => B !> ≡ <! ¬ (A ∧ ¬ B) !>.
+    <! A ⇒ B !> ≡ <! ¬ (A ∧ ¬ B) !>.
   Proof. prove_equiv. Qed.
 
   (* A.25 *)
   Lemma f_not_impl A B :
-      <! ¬ (A => B) !> ≡ <! A ∧ ¬ B !>.
+      <! ¬ (A ⇒ B) !> ≡ <! A ∧ ¬ B !>.
   Proof. prove_equiv. Qed.
 
   (* A.26 *)
   Lemma f_contrapositive A B :
-      <! A => B !> ≡ <! ¬ B => ¬ A !>.
+      <! A ⇒ B !> ≡ <! ¬ B ⇒ ¬ A !>.
   Proof. prove_equiv. Qed.
 
   (* A.27 *)
   Lemma f_implies_true A :
-    <! A => true !> ≡ <! true !>.
+    <! A ⇒ true !> ≡ <! true !>.
   Proof. prove_equiv. Qed.
 
   (* A.28 *)
   Lemma f_true_implies A :
-      <! true => A !> ≡ <! A !>.
+      <! true ⇒ A !> ≡ <! A !>.
   Proof. prove_equiv. Qed.
 
   (* A.29 *)
   Lemma f_implies_false A :
-    <! A => false !> ≡ <! ¬ A !>.
+    <! A ⇒ false !> ≡ <! ¬ A !>.
   Proof. prove_equiv. Qed.
 
   (* A.30 *)
   Lemma f_false_implies A :
-      <! false => A !> ≡ <! true !>.
+      <! false ⇒ A !> ≡ <! true !>.
   Proof. prove_equiv. Qed.
 
   (* A.31 *)
   Lemma f_implies_not_self A :
-      <! A => ¬ A !> ≡ <! ¬ A !>.
+      <! A ⇒ ¬ A !> ≡ <! ¬ A !>.
   Proof. prove_equiv. Qed.
 
   (* A.32 *)
   Lemma f_not_implies_self A :
-      <! ¬ A => A !> ≡ <! A !>.
+      <! ¬ A ⇒ A !> ≡ <! A !>.
   Proof. prove_equiv. Qed.
 
   (* A.33 *)
   Lemma f_impl_distr1 A B C :
-      <! C => (A ∧ B) !> ≡ <! (C => A) ∧ (C => B) !>.
+      <! C ⇒ (A ∧ B) !> ≡ <! (C ⇒ A) ∧ (C ⇒ B) !>.
   Proof. prove_equiv. Qed.
 
   (* A.34 *)
   Lemma f_impl_distr2 A B C :
-    <! (A ∨ B) => C !> ≡ <! (A => C) ∧ (B => C) !>.
+    <! (A ∨ B) ⇒ C !> ≡ <! (A ⇒ C) ∧ (B ⇒ C) !>.
   Proof. prove_equiv. Qed.
 
   (* A.35 *)
   Lemma f_impl_distr3 A B C :
-    <! C => (A ∨ B) !> ≡ <! (C => A) ∨ (C => B) !>.
+    <! C ⇒ (A ∨ B) !> ≡ <! (C ⇒ A) ∨ (C ⇒ B) !>.
   Proof. prove_equiv. Qed.
 
   (* A.36 *)
   Lemma f_impl_distr4 A B C :
-    <! (A ∧ B) => C !> ≡ <! (A => C) ∨ (B => C) !>.
+    <! (A ∧ B) ⇒ C !> ≡ <! (A ⇒ C) ∨ (B ⇒ C) !>.
   Proof with auto.
     unfold FImpl. intros σ. simp feval. split; [| naive_solver].
     intros [|]... apply Decidable.not_and in H as [|]... apply feval_dec.
   Qed.
 
   (* A.37 *)
-  Lemma f_successive_hypotheses A B C :
-    <! A => (B => C) !> ≡ <! (A ∧ B) => C !>.
-  Proof with auto.
-    unfold FImpl. intros σ. simp feval. split; [naive_solver |].
-    intros [|]... apply Decidable.not_and in H as [|]... apply feval_dec.
-  Qed.
-
-  (* A.37 *)
-  Lemma f_successive_hypotheses' A B C :
-    <! B => (A => C) !> ≡ <! (A ∧ B) => C !>.
+  Lemma f_impl_curry A B C :
+    <! A ⇒ (B ⇒ C) !> ≡ <! (A ∧ B) ⇒ C !>.
   Proof with auto.
     unfold FImpl. intros σ. simp feval. split; [naive_solver |].
     intros [|]... apply Decidable.not_and in H as [|]... apply feval_dec.
   Qed.
 
   (* A.38 *)
-  Lemma f_def_by_cases A B C :
-    <! (A => B) ∧ (¬A => C) !> ≡ <! (A ∧ B) ∨ (¬A ∧ C) !>.
+  Lemma f_cases_as_or A B C :
+    <! (A ⇒ B) ∧ (¬A ⇒ C) !> ≡ <! (A ∧ B) ∨ (¬A ∧ C) !>.
   Proof. prove_equiv. Qed.
 
   (* A.39 *)
   Lemma f_iff_as_and A B C :
-    <! A <=> B !> ≡ <! (A => B) ∧ (B => A) !>.
+    <! A ⇔ B !> ≡ <! (A ⇒ B) ∧ (B ⇒ A) !>.
   Proof. prove_equiv. Qed.
 
   (* A.40 *)
   Lemma f_iff_as_or A B :
-    <! A <=> B !> ≡ <! (A ∧ B) ∨ ¬(A ∨ B) !>.
+    <! A ⇔ B !> ≡ <! (A ∧ B) ∨ ¬(A ∨ B) !>.
   Proof. prove_equiv. Qed.
 
   (* A.41 *)
   Lemma f_iff_negate A B :
-    <! A <=> B !> ≡ <! ¬A <=> ¬B !>.
+    <! A ⇔ B !> ≡ <! ¬A ⇔ ¬B !>.
   Proof. prove_equiv. Qed.
 
   (* A.42 *)
   Lemma f_iff_self A :
-    <! A <=> A !> ≡ <! true !>.
+    <! A ⇔ A !> ≡ <! true !>.
   Proof. prove_equiv. Qed.
 
   (* A.43 *)
   Lemma f_iff_not_self A :
-    <! A <=> ¬ A !> ≡ <! false !>.
+    <! A ⇔ ¬ A !> ≡ <! false !>.
   Proof. prove_equiv. Qed.
 
   (* A.44 *)
   Lemma f_iff_true A :
-    <! A <=> true !> ≡ <! A !>.
+    <! A ⇔ true !> ≡ <! A !>.
   Proof. prove_equiv. Qed.
 
   (* A.45 *)
   Lemma f_iff_false A :
-    <! A <=> false !> ≡ <! ¬ A !>.
+    <! A ⇔ false !> ≡ <! ¬ A !>.
   Proof. prove_equiv. Qed.
 
   (* A.46 *)
   Lemma f_iff_and_absorb A B :
-    <! A <=> (A ∧ B) !> ≡ <! A => B !>.
+    <! A ⇔ (A ∧ B) !> ≡ <! A ⇒ B !>.
   Proof. prove_equiv. Qed.
 
   (* A.47 *)
   Lemma f_iff_or_absorb A B :
-    <! A <=> (A ∨ B) !> ≡ <! B => A !>.
+    <! A ⇔ (A ∨ B) !> ≡ <! B ⇒ A !>.
   Proof with auto.
     intros σ. unfold FIff, FImpl. simp feval. split.
     - intros []. destruct_or! H; naive_solver.
@@ -260,7 +252,7 @@ Section props.
 
   (* A.48 *)
   Lemma f_or_iff A B C :
-    <! A ∨ (B <=> C) !> ≡ <! (A ∨ B) <=> (A ∨ C) !>.
+    <! A ∨ (B ⇔ C) !> ≡ <! (A ∨ B) ⇔ (A ∨ C) !>.
   Proof with auto.
     intros σ. unfold FIff, FImpl. simp feval. split; [|naive_solver].
     intros [|[]]; [naive_solver|]. split; destruct (feval_lem σ A); naive_solver.
@@ -268,12 +260,12 @@ Section props.
 
   (* A.49 *)
   Lemma f_iff_comm A B :
-    <! A <=> B !> ≡ <! B <=> A !>.
+    <! A ⇔ B !> ≡ <! B ⇔ A !>.
   Proof. prove_equiv. Qed.
 
   (* A.50 *)
   Lemma f_iff_assoc A B C :
-      <! A <=> (B <=> C) !> ≡ <! (A <=> B) <=> C !>.
+      <! A ⇔ (B ⇔ C) !> ≡ <! (A ⇔ B) ⇔ C !>.
   Proof.
     unfold FIff, FImpl. rewrite f_not_and.
     repeat rewrite f_not_and. repeat rewrite f_not_or. repeat rewrite f_not_stable.
@@ -283,10 +275,10 @@ Section props.
   (* A.56 *)
   Lemma f_exists_one_point x t A :
       x ∉ term_fvars t →
-      <! exists x, x = t ∧ A !> ≡ <! A[x \ t] !>.
+      <! ∃ x, ⌜x = t⌝ ∧ A !> ≡ <! A[x \ t] !>.
   Proof with auto.
     intros Hfree σ. simp feval. setoid_rewrite simpl_subst_and.
-    setoid_rewrite simpl_subst_sf. simpl. destruct (decide (x = x)); [|contradiction].
+    setoid_rewrite simpl_subst_af. simpl. destruct (decide (x = x)); [|contradiction].
     clear e. split.
     - intros [v Hv]. simp feval in Hv. destruct Hv as [H1 H2]. inversion H1.
       destruct H as []. inversion H. subst v0 x0. clear H H1.
@@ -303,7 +295,7 @@ Section props.
   (* A.56 *)
   Lemma f_forall_one_point x t A :
       x ∉ term_fvars t →
-      <! forall x, x = t => A !> ≡ <! A[x \ t] !>.
+      <! ∀ x, ⌜x = t⌝ ⇒ A !> ≡ <! A[x \ t] !>.
   Proof with auto.
     intros Hfree. unfold FForall. rewrite f_not_impl.
     apply (f_exists_one_point x t(FNot A)) in Hfree. rewrite Hfree.
@@ -312,27 +304,27 @@ Section props.
 
   (* A.60 *)
   Lemma f_exists_idemp x A :
-    <! exists x x, A !> ≡ <! exists x, A !>.
+    <! ∃ x x, A !> ≡ <! ∃ x, A !>.
   Proof with auto. rewrite fexists_unused... simpl. set_solver. Qed.
 
   (* A.59 *)
   Lemma f_forall_idemp x A :
-    <! forall x x, A !> ≡ <! forall x, A !>.
+    <! ∀ x x, A !> ≡ <! ∀ x, A !>.
   Proof with auto. unfold FForall. rewrite f_not_stable. rewrite f_exists_idemp... Qed.
 
   (* A.61 *)
   Lemma f_not_forall x A :
-    <! ¬ forall x, A !> ≡ <! exists x, ¬ A !>.
+    <! ¬ ∀ x, A !> ≡ <! ∃ x, ¬ A !>.
   Proof. unfold FForall. rewrite f_not_stable. auto. Qed.
 
   (* A.62 *)
   Lemma f_not_exists x A :
-    <! ¬ exists x, A !> ≡ <! forall x, ¬ A !>.
+    <! ¬ ∃ x, A !> ≡ <! ∀ x, ¬ A !>.
   Proof. unfold FForall. rewrite f_not_stable. auto. Qed.
 
   (* A.64 *)
   Lemma f_exists_comm x y A :
-    <! exists x y, A !> ≡ <! exists y x, A !>.
+    <! ∃ x y, A !> ≡ <! ∃ y x, A !>.
   Proof with auto.
     intros σ. destruct (decide (x = y)). 1:{ subst... }
     destruct (decide (x ∈ formula_fvars A)).
@@ -353,12 +345,12 @@ Section props.
 
   (* A.63 *)
   Lemma f_forall_comm x y A :
-    <! forall x y, A !> ≡ <! forall y x, A !>.
+    <! ∀ x y, A !> ≡ <! ∀ y x, A !>.
   Proof. unfold FForall. do 2 rewrite f_not_stable. rewrite f_exists_comm. reflexivity. Qed.
 
   (* A.66 *)
   Lemma f_exists_or x A B :
-    <! exists x, A ∨ B !> ≡ <! (exists x, A) ∨ (exists x, B) !>.
+    <! ∃ x, A ∨ B !> ≡ <! (∃ x, A) ∨ (∃ x, B) !>.
   Proof with auto.
     intros σ. simp feval. setoid_rewrite simpl_subst_or. split.
     - intros [v H]. simp feval in H. destruct H as [|]; [left|right]; exists v...
@@ -367,19 +359,19 @@ Section props.
 
   (* A.65 *)
   Lemma f_forall_and x A B :
-    <! forall x, A ∧ B !> ≡ <! (forall x, A) ∧ (forall x, B) !>.
+    <! ∀ x, A ∧ B !> ≡ <! (∀ x, A) ∧ (∀ x, B) !>.
   Proof. unfold FForall. rewrite f_not_and. rewrite f_exists_or. rewrite f_not_or; auto. Qed.
 
   (* A.67 *)
   Lemma f_exists_impl x A B :
-    <! exists x, A => B !> ≡ <! (forall x, A) => (exists x, B) !>.
+    <! ∃ x, A ⇒ B !> ≡ <! (∀ x, A) ⇒ (∃ x, B) !>.
   Proof with auto.
     intros σ. unfold FImpl. rewrite f_exists_or. unfold FForall. rewrite f_not_stable...
   Qed.
 
   (* A.68 *)
   Lemma f_forall_ent_exists x A :
-    <! forall x, A !> ⇛ <! exists x, A !>.
+    <! ∀ x, A !> ⇛ <! ∃ x, A !>.
   Proof.
     intros σ. rewrite simpl_feval_fforall. intros. simp feval.
     exists ⊥. apply H.
@@ -387,7 +379,7 @@ Section props.
 
   (* A.69 *)
   Lemma f_or_forall x A B :
-    <! (forall x, A) ∨ (forall x, B) !> ⇛ <! forall x, A ∨ B !>.
+    <! (∀ x, A) ∨ (∀ x, B) !> ⇛ <! ∀ x, A ∨ B !>.
   Proof.
     intros σ. simp feval. do 3 rewrite simpl_feval_fforall.
     setoid_rewrite simpl_subst_or.
@@ -396,7 +388,7 @@ Section props.
 
   (* A.70 *)
   Lemma f_forall_impl x A B :
-    <! forall x, A => B !> ⇛ <! (forall x, A) => (forall x, B) !>.
+    <! ∀ x, A ⇒ B !> ⇛ <! (∀ x, A) ⇒ (∀ x, B) !>.
   Proof.
     intros σ. rewrite simpl_feval_fimpl. do 3 rewrite simpl_feval_fforall.
     intros. specialize (H v). rewrite simpl_subst_impl in H. rewrite simpl_feval_fimpl in H.
@@ -405,7 +397,7 @@ Section props.
 
   (* A.71 *)
   Lemma f_exists_and x A B :
-    <! exists x, A ∧ B !> ⇛ <! (exists x, A) ∧ (exists x, B) !>.
+    <! ∃ x, A ∧ B !> ⇛ <! (∃ x, A) ∧ (∃ x, B) !>.
   Proof with auto.
     intros σ. simp feval. intros [v H]. rewrite simpl_subst_and in H. simp feval in H.
     destruct H as []. split; exists v...
@@ -413,18 +405,18 @@ Section props.
 
   (* A.72 *)
   Lemma f_impl_exists x A B :
-    <! (exists x, A) => (exists x, B) !> ⇛ <! exists x, A => B !>.
+    <! (∃ x, A) ⇒ (∃ x, B) !> ⇛ <! ∃ x, A ⇒ B !>.
   Proof with auto.
     intros σ. rewrite simpl_feval_fimpl. intros. simp feval.
     setoid_rewrite simpl_subst_impl. setoid_rewrite simpl_feval_fimpl.
-    destruct (feval_lem σ <! exists x, A !>).
+    destruct (feval_lem σ <! ∃ x, A !>).
     - apply H in H0. simp feval in H0. destruct H0 as [v Hv]. exists v. intros...
     - exists ⊥. intros. simp feval in H0. exfalso. apply H0. exists ⊥...
   Qed.
 
   (* A.73 *)
   Lemma f_exists_forall x y A :
-    <! exists x, (forall y, A) !> ⇛ <! forall y, (exists x, A) !>.
+    <! ∃ x, (∀ y, A) !> ⇛ <! ∀ y, (∃ x, A) !>.
   Proof with auto.
     intros σ. simp feval. rewrite simpl_feval_fforall. intros [vx H] vy.
     destruct (decide (x = y)).
@@ -442,19 +434,19 @@ Section props.
   (* A.76 *)
   Lemma f_forall_and_unused_l x A B :
     x ∉ formula_fvars A →
-    <! forall x, A ∧ B !> ≡ <! A ∧ (forall x, B) !>.
+    <! ∀ x, A ∧ B !> ≡ <! A ∧ (∀ x, B) !>.
   Proof with auto. intros. rewrite f_forall_and. rewrite fforall_unused... Qed.
 
   (* A.76' *)
   Lemma f_forall_and_unused_r x A B :
     x ∉ formula_fvars B →
-    <! forall x, A ∧ B !> ≡ <! (forall x, A) ∧ B !>.
+    <! ∀ x, A ∧ B !> ≡ <! (∀ x, A) ∧ B !>.
   Proof with auto. intros. rewrite f_forall_and. rewrite (fforall_unused x B)... Qed.
 
   (* A.77 *)
   Lemma f_forall_or_unused_l x A B :
     x ∉ formula_fvars A →
-    <! forall x, A ∨ B !> ≡ <! A ∨ (forall x, B) !>.
+    <! ∀ x, A ∨ B !> ≡ <! A ∨ (∀ x, B) !>.
   Proof with auto.
     intros. intros σ. rewrite simpl_feval_fforall. setoid_rewrite simpl_subst_or.
     split; intros.
@@ -469,7 +461,7 @@ Section props.
   (* A.77' *)
   Lemma f_forall_or_unused_r x A B :
     x ∉ formula_fvars B →
-    <! forall x, A ∨ B !> ≡ <! (forall x, A) ∨ B !>.
+    <! ∀ x, A ∨ B !> ≡ <! (∀ x, A) ∨ B !>.
   Proof with auto.
     intros. intros σ. rewrite simpl_feval_fforall. setoid_rewrite simpl_subst_or.
     split; intros.
@@ -485,7 +477,7 @@ Section props.
   (* A.78 *)
   Lemma f_forall_impl_unused_l x A B :
     x ∉ formula_fvars A →
-    <! forall x, A => B !> ≡ <! A => (forall x, B) !>.
+    <! ∀ x, A ⇒ B !> ≡ <! A ⇒ (∀ x, B) !>.
   Proof with auto.
     intros. intros σ. rewrite simpl_feval_fforall. setoid_rewrite simpl_subst_impl.
     rewrite simpl_feval_fimpl.
@@ -500,7 +492,7 @@ Section props.
   (* A.79 *)
   Lemma f_forall_impl_unused_r x A B :
     x ∉ formula_fvars B →
-    <! forall x, A => B !> ≡ <! (exists x, A) => B !>.
+    <! ∀ x, A ⇒ B !> ≡ <! (∃ x, A) ⇒ B !>.
   Proof with auto.
     intros. intros σ. rewrite simpl_feval_fforall. setoid_rewrite simpl_subst_impl.
     setoid_rewrite simpl_feval_fimpl. simp feval.
@@ -513,7 +505,7 @@ Section props.
   (* A.80 *)
   Lemma f_exists_and_unused_l x A B :
     x ∉ formula_fvars A →
-    <! exists x, A ∧ B !> ≡ <! A ∧ (exists x, B) !>.
+    <! ∃ x, A ∧ B !> ≡ <! A ∧ (∃ x, B) !>.
   Proof with auto.
     intros. rewrite <- (f_not_stable A). rewrite <- (f_not_stable B). rewrite <- (f_not_or).
     rewrite <- (f_not_forall). rewrite f_forall_or_unused_l by (simpl; auto).
@@ -523,7 +515,7 @@ Section props.
   (* A.80' *)
   Lemma f_exists_and_unused_r x A B :
     x ∉ formula_fvars B →
-    <! exists x, A ∧ B !> ≡ <! (exists x, A) ∧ B !>.
+    <! ∃ x, A ∧ B !> ≡ <! (∃ x, A) ∧ B !>.
   Proof with auto.
     intros. rewrite <- (f_not_stable A). rewrite <- (f_not_stable B). rewrite <- (f_not_or).
     rewrite <- (f_not_forall). rewrite f_forall_or_unused_r by (simpl; auto).
@@ -533,25 +525,25 @@ Section props.
   (* A.81 *)
   Lemma f_exists_or_unused_l x A B :
     x ∉ formula_fvars A →
-    <! exists x, A ∨ B !> ≡ <! A ∨ (exists x, B) !>.
+    <! ∃ x, A ∨ B !> ≡ <! A ∨ (∃ x, B) !>.
   Proof with auto. intros. rewrite f_exists_or. rewrite fexists_unused... Qed.
 
   (* A.81' *)
   Lemma f_exists_or_unused_r x A B :
     x ∉ formula_fvars B →
-    <! exists x, A ∨ B !> ≡ <! (exists x, A) ∨ B !>.
+    <! ∃ x, A ∨ B !> ≡ <! (∃ x, A) ∨ B !>.
   Proof with auto. intros. rewrite f_exists_or. rewrite (fexists_unused _ B)... Qed.
 
   (* A.82 *)
   Lemma f_exists_impl_unused_l x A B :
     x ∉ formula_fvars A →
-    <! exists x, A => B !> ≡ <! A => (exists x, B) !>.
+    <! ∃ x, A ⇒ B !> ≡ <! A ⇒ (∃ x, B) !>.
   Proof with auto. intros. rewrite f_exists_impl. rewrite fforall_unused... Qed.
 
   (* A.83 *)
   Lemma f_exists_impl_unused_r x A B :
     x ∉ formula_fvars B →
-    <! exists x, A => B !> ≡ <! (forall x, A) => B !>.
+    <! ∃ x, A ⇒ B !> ≡ <! (∀ x, A) ⇒ B !>.
   Proof with auto. intros. rewrite f_exists_impl. rewrite fexists_unused... Qed.
 
   (* A.84: fforall_alpha_equiv *)
@@ -559,7 +551,7 @@ Section props.
 
   (* A.86 *)
   Lemma f_forall_elim t x A :
-    <! forall x, A !> ⇛ A[x \ t].
+    <! ∀ x, A !> ⇛ A[x \ t].
   Proof with auto.
     intros σ. rewrite simpl_feval_fforall. intros. pose proof (teval_total σ t) as [v Hv].
     specialize (H v). rewrite (feval_subst v) in H... rewrite (feval_subst v)...
@@ -567,14 +559,14 @@ Section props.
 
   (* A.86 *)
   Lemma f_exists_intro t x A :
-    A[x \ t] ⇛ <! exists x, A !>.
+    A[x \ t] ⇛ <! ∃ x, A !>.
   Proof with auto.
     intros σ. simp feval. intros. pose proof (teval_total σ t) as [v Hv].
     exists v. rewrite (feval_subst v) in H... rewrite (feval_subst v)...
   Qed.
 
   Lemma f_impl_elim A B :
-    <! A ∧ (A => B) !> ⇛ B.
+    <! A ∧ (A ⇒ B) !> ⇛ B.
   Proof with auto.
     intros σ. simp feval. rewrite simpl_feval_fimpl. naive_solver.
   Qed.
@@ -598,11 +590,11 @@ Section props.
   Proof. intros. rewrite H. reflexivity. Qed.
 
   Lemma f_impl_cancel_l A B C :
-    B ≡ C → <! A => B !> ≡ <! A => C !>.
+    B ≡ C → <! A ⇒ B !> ≡ <! A ⇒ C !>.
   Proof. intros. rewrite H. reflexivity. Qed.
 
   Lemma f_impl_cancel_r A B C :
-    B ≡ C → <! B => A !> ≡ <! C => A !>.
+    B ≡ C → <! B ⇒ A !> ≡ <! C ⇒ A !>.
   Proof. intros. rewrite H. reflexivity. Qed.
 
   Lemma f_subst_cancel A B x t :
@@ -615,12 +607,12 @@ Section props.
 
   Lemma f_exists_equiv A B y1 y2 :
     (∀ t, A[y1 \ t] ≡ B[y2 \ t]) →
-    <! exists y1, A !> ≡ <! exists y2, B !>.
+    <! ∃ y1, A !> ≡ <! ∃ y2, B !>.
   Proof. intros Hequiv σ. apply feval_exists_equiv_if. naive_solver. Qed.
 
   Lemma f_forall_equiv A B y1 y2 :
     (∀ t, A[y1 \ t] ≡ B[y2 \ t]) →
-    <! forall y1, A !> ≡ <! forall y2, B !>.
+    <! ∀ y1, A !> ≡ <! ∀ y2, B !>.
   Proof. intros Hequiv σ. do 2 rewrite simpl_feval_fforall. naive_solver. Qed.
 
   Lemma f_ent_and_cancel_l A B C :
@@ -647,36 +639,47 @@ Section props.
   Qed.
 
   Lemma f_ent_impl_cancel_l A B C :
-    B ⇛ C → <! A => B !> ⇛ <! A => C !>.
+    B ⇛ C → <! A ⇒ B !> ⇛ <! A ⇒ C !>.
   Proof. intros H σ. do 2 rewrite simpl_feval_fimpl. naive_solver. Qed.
 
   Lemma f_ent_impl_cancel_r A B C :
-    C ⇛ B → <! B => A !> ⇛ <! C => A !>.
+    C ⇛ B → <! B ⇒ A !> ⇛ <! C ⇒ A !>.
   Proof. intros H σ. do 2 rewrite simpl_feval_fimpl. naive_solver. Qed.
 
   Lemma f_exists_ent A B y1 y2 :
     (∀ t, A[y1 \ t] ⇛ B[y2 \ t]) →
-    <! exists y1, A !> ⇛ <! exists y2, B !>.
+    <! ∃ y1, A !> ⇛ <! ∃ y2, B !>.
   Proof.
     intros Hequiv σ. simp feval. intros [v Hv]. exists v. naive_solver.
   Qed.
 
   Lemma f_forall_ent A B y1 y2 :
     (∀ t, A[y1 \ t] ⇛ B[y2 \ t]) →
-    <! forall y1, A !> ⇛ <! forall y2, B !>.
+    <! ∀ y1, A !> ⇛ <! ∀ y2, B !>.
   Proof.
     intros Hequiv σ. do 2 rewrite simpl_feval_fforall. intros. naive_solver.
   Qed.
 
   Lemma f_ent_elim σ A B :
-    σ ⊨ A →
+    feval σ A →
     A ⇛ B →
-    σ ⊨ B.
+    feval σ B.
   Proof. naive_solver. Qed.
 
   Lemma f_ent_intro A B :
-    (∀ σ, σ ⊨ A → σ ⊨ B) →
+    (∀ σ, feval σ A → feval σ B) →
     A ⇛ B.
   Proof. naive_solver. Qed.
 
+  Lemma f_eq_refl t :
+    <! ⌜t = t⌝ !> ≡ <! true !>.
+  Proof.
+    prove_equiv. intros. destruct (teval_total σ t) as [v Hv]. econstructor. split; exact Hv.
+  Qed.
+
+  Lemma f_neq_irrefl t :
+    <! ⌜t ≠ t⌝ !> ≡ <! false !>.
+  Proof.
+    rewrite f_eq_refl. rewrite f_not_true. reflexivity.
+  Qed.
 End props.
